Refactor to avoid dlist

Locally_Nameless_Lambda_Calculus/LN_Lambda_Typing.thy
@@ -1,6 +1,5 @@
 theory LN_Lambda_Typing
   imports
-    "HOL-Library.Dlist"
     LN_Lambda_Term
     "Abstract_Substitution.Substitution"
 begin
@@ -449,25 +448,27 @@ qed *)
 
 section \<open>Type System\<close>
 
-type_synonym ('\<V>\<^sub>t\<^sub>y, '\<Sigma>\<^sub>t\<^sub>y) pre_const_ty = "'\<V>\<^sub>t\<^sub>y dlist \<times> ('\<V>\<^sub>t\<^sub>y, '\<Sigma>\<^sub>t\<^sub>y) ty list \<times> ('\<V>\<^sub>t\<^sub>y, '\<Sigma>\<^sub>t\<^sub>y) ty"
+type_synonym ('\<V>\<^sub>t\<^sub>y, '\<Sigma>\<^sub>t\<^sub>y) pre_const_ty = "'\<V>\<^sub>t\<^sub>y list \<times> ('\<V>\<^sub>t\<^sub>y, '\<Sigma>\<^sub>t\<^sub>y) ty list \<times> ('\<V>\<^sub>t\<^sub>y, '\<Sigma>\<^sub>t\<^sub>y) ty"
 
-text \<open>A constant's declared type-variable tuple must contain every type variable occurring in its
-  parameter and result types, matching the paper's signature well-formedness requirement.\<close>
+text \<open>A constant's declared type-variable tuple must be distinct and must contain every type
+  variable occurring in its parameter and result types, matching the paper's signature
+  well-formedness requirement.\<close>
 
 definition wf_const_ty :: "('\<V>\<^sub>t\<^sub>y, '\<Sigma>\<^sub>t\<^sub>y :: arity) pre_const_ty \<Rightarrow> bool" where
-  "wf_const_ty \<equiv> \<lambda>(\<alpha>s, \<tau>s, \<tau>). (\<Union>\<tau>'\<in>set \<tau>s. type_vars \<tau>') \<union> type_vars \<tau> \<subseteq> set (list_of_dlist \<alpha>s)"
+  "wf_const_ty \<equiv> \<lambda>(\<alpha>s, \<tau>s, \<tau>).
+    distinct \<alpha>s \<and> (\<Union>\<tau>'\<in>set \<tau>s. type_vars \<tau>') \<union> type_vars \<tau> \<subseteq> set \<alpha>s"
 
 typedef (overloaded) ('\<V>\<^sub>t\<^sub>y, '\<Sigma>\<^sub>t\<^sub>y :: arity) const_ty =
   \<open>{c :: ('\<V>\<^sub>t\<^sub>y, '\<Sigma>\<^sub>t\<^sub>y) pre_const_ty. wf_const_ty c}\<close>
 proof
-  show \<open>(Dlist.Dlist [undefined], [], TyVar undefined) \<in> {c. wf_const_ty c}\<close>
+  show \<open>([undefined], [], TyVar undefined) \<in> {c. wf_const_ty c}\<close>
     by (simp add: wf_const_ty_def)
 qed
 
 setup_lifting type_definition_const_ty
 
 definition ConstTy ::
-  "'\<V>\<^sub>t\<^sub>y dlist \<Rightarrow> ('\<V>\<^sub>t\<^sub>y, '\<Sigma>\<^sub>t\<^sub>y) ty list \<Rightarrow> ('\<V>\<^sub>t\<^sub>y, '\<Sigma>\<^sub>t\<^sub>y) ty \<Rightarrow> ('\<V>\<^sub>t\<^sub>y, '\<Sigma>\<^sub>t\<^sub>y :: arity) const_ty" where
+  "'\<V>\<^sub>t\<^sub>y list \<Rightarrow> ('\<V>\<^sub>t\<^sub>y, '\<Sigma>\<^sub>t\<^sub>y) ty list \<Rightarrow> ('\<V>\<^sub>t\<^sub>y, '\<Sigma>\<^sub>t\<^sub>y) ty \<Rightarrow> ('\<V>\<^sub>t\<^sub>y, '\<Sigma>\<^sub>t\<^sub>y :: arity) const_ty" where
   "wf_const_ty (\<alpha>s, \<tau>s, \<tau>) \<Longrightarrow> ConstTy \<alpha>s \<tau>s \<tau> = Abs_const_ty (\<alpha>s, \<tau>s, \<tau>)"
 
 lemma Rep_const_ty_ConstTy[simp]:
@@ -480,8 +481,8 @@ inductive has_type ::
     (('\<V>\<^sub>t\<^sub>y, '\<Sigma>\<^sub>t\<^sub>y) ty, '\<Sigma>, '\<V>) preterm \<Rightarrow> ('\<V>\<^sub>t\<^sub>y, '\<Sigma>\<^sub>t\<^sub>y) ty \<Rightarrow> bool"
   for \<C> where
   Const: "has_type \<C> (Const c \<tau>\<^sub>1s ts) \<tau>"
-    if "Rep_const_ty (\<C> c) = (\<alpha>s, \<tau>\<^sub>2s, \<tau>\<^sub>3)" and "Dlist.length \<alpha>s = length \<tau>\<^sub>1s" and
-      "\<sigma> = fun_upds TyVar (list_of_dlist \<alpha>s) \<tau>\<^sub>1s" and
+    if "Rep_const_ty (\<C> c) = (\<alpha>s, \<tau>\<^sub>2s, \<tau>\<^sub>3)" and "length \<alpha>s = length \<tau>\<^sub>1s" and
+      "\<sigma> = fun_upds TyVar \<alpha>s \<tau>\<^sub>1s" and
       "list_all2 (has_type \<C>) ts (map (\<lambda>\<tau>\<^sub>2. \<tau>\<^sub>2 \<cdot>\<^sub>t\<^sub>y \<sigma>) \<tau>\<^sub>2s)" and
       "\<tau> = \<tau>\<^sub>3 \<cdot>\<^sub>t\<^sub>y \<sigma>"
     for c \<tau>\<^sub>1s ts \<tau> |
@@ -565,8 +566,8 @@ proof (induction t \<tau>\<^sub>1 rule: has_type.induct)
     unfolding subst_free.simps
   proof (rule has_type.Const)
     show "Rep_const_ty (\<C> c) = (\<alpha>s, \<tau>\<^sub>2s, \<tau>\<^sub>3)" by (rule Const.hyps(1))
-    show "Dlist.length \<alpha>s = length \<tau>\<^sub>1s" by (rule Const.hyps(2))
-    show "\<sigma> = fun_upds TyVar (list_of_dlist \<alpha>s) \<tau>\<^sub>1s" by (rule Const.hyps(3))
+    show "length \<alpha>s = length \<tau>\<^sub>1s" by (rule Const.hyps(2))
+    show "\<sigma> = fun_upds TyVar \<alpha>s \<tau>\<^sub>1s" by (rule Const.hyps(3))
     show "list_all2 (has_type \<C>) ts (map (\<lambda>\<tau>\<^sub>2. \<tau>\<^sub>2 \<cdot>\<^sub>t\<^sub>y \<sigma>) \<tau>\<^sub>2s)"
       by (rule list.rel_mono_strong[OF Const.IH]) simp
     show "\<tau> = \<tau>\<^sub>3 \<cdot>\<^sub>t\<^sub>y \<sigma>" by (rule Const.hyps(4))
